Weidenbach_Book/IsaSAT/IsaSAT_EMA.thy
@@ -4,8 +4,11 @@ begin
 
 section \<open>Moving averages\<close>
 
+definition EMA_FIXPOINT_SIZE :: \<open>nat\<close> where
+  \<open>EMA_FIXPOINT_SIZE = 32\<close>
+
 text \<open>We use (at least hopefully) the variant of EMA-14 implemented in Cadical, but with fixed-point
-calculations (\<^term>\<open>1 :: nat\<close> is \<^term>\<open>(1 :: nat) >> 32\<close>).
+calculations (\<^term>\<open>1 :: nat\<close> is \<^term>\<open>(1 :: nat) >> EMA_FIXPOINT_SIZE\<close>).
 
 Remark that the coefficient \<^term>\<open>\<beta>\<close> already should take care of the fixed-point conversion of the glue.
 Otherwise, \<^term>\<open>value\<close> is wrongly updated.
@@ -13,15 +16,21 @@ Otherwise, \<^term>\<open>value\<close> is wrongly updated.
 type_synonym ema = \<open>64 word \<times> 64 word \<times> 64 word \<times> 64 word \<times> 64 word\<close>
 
 definition ema_bitshifting where
-  \<open>ema_bitshifting = (1 << 32)\<close>
+  \<open>ema_bitshifting = (1 << EMA_FIXPOINT_SIZE)\<close>
+
+
+definition EMA_MULT_SHIFT :: \<open>nat\<close> where
+  \<open>EMA_MULT_SHIFT = 8\<close>
 
 text \<open>TODO: some precision is lost  here in the difference calculation.\<close>
 definition (in -) ema_update :: \<open>nat \<Rightarrow> ema \<Rightarrow> ema\<close> where
   \<open>ema_update = (\<lambda>lbd (value, \<alpha>, \<beta>, wait, period).
      let lbd = (of_nat lbd) * ema_bitshifting in
-     let value = if lbd > value then value + ((\<beta> >> 24) * ((lbd - value) >> 8))
-                                else value - ((\<beta> >> 24) * ((value - lbd) >> 8)) in
-     if \<beta> \<le> \<alpha> \<or> wait > 0 then (value, \<alpha>, \<beta>, wait - 1, period)
+     let value = if lbd > value
+        then value + ((\<beta> >> (EMA_FIXPOINT_SIZE - EMA_MULT_SHIFT)) * ((lbd - value) >> EMA_MULT_SHIFT))
+        else value - ((\<beta> >> (EMA_FIXPOINT_SIZE - EMA_MULT_SHIFT)) * ((value - lbd) >> EMA_MULT_SHIFT))
+     in
+       if \<beta> \<le> \<alpha> \<or> wait > 0 then (value, \<alpha>, \<beta>, wait - 1, period)
      else
        let wait = 2 * period + 1 in
        let period = wait in
@@ -30,7 +39,7 @@ definition (in -) ema_update :: \<open>nat \<Rightarrow> ema \<Rightarrow> ema\<
        (value, \<alpha>, \<beta>, wait, period))\<close>
 
 definition (in -) ema_init :: \<open>64 word \<Rightarrow> ema\<close> where
-  \<open>ema_init \<alpha> = (0, \<alpha>, ema_bitshifting, 0, 0)\<close>
+  \<open>ema_init \<alpha> = (0, \<alpha>  >> (EMA_FIXPOINT_SIZE - 32), ema_bitshifting, 0, 0)\<close>
 
 fun ema_reinit where
   \<open>ema_reinit (value, \<alpha>, \<beta>, wait, period) = (value, \<alpha>, ema_bitshifting, 0, 0)\<close>
@@ -39,22 +48,25 @@ fun ema_get_value :: \<open>ema \<Rightarrow> 64 word\<close> where
   \<open>ema_get_value (v, _) = v\<close>
 
 fun ema_extract_value :: \<open>ema \<Rightarrow> 64 word\<close> where
-  \<open>ema_extract_value (v, _) = v >> 32\<close>
+  \<open>ema_extract_value (v, _) = v >> EMA_FIXPOINT_SIZE\<close>
 
 
 text \<open>We use the default values for Cadical: \<^term>\<open>(3 / 10 ^2)\<close> and  \<^term>\<open>(1 / 10 ^ 5)\<close>  in our fixed-point
   version.
 \<close>
-
+value \<open>((3 :: 64 word) << EMA_FIXPOINT_SIZE) >> (15)\<close>
+value \<open>((4 :: 64 word) << EMA_FIXPOINT_SIZE >> 7)\<close>
 abbreviation ema_fast_init :: ema where
-  \<open>ema_fast_init \<equiv> ema_init (128849010)\<close>
+  \<open>ema_fast_init \<equiv> ema_init (128849010)\<close> \<comment> \<open>5629499534213\<close>
 
 abbreviation ema_slow_init :: ema where
-  \<open>ema_slow_init \<equiv> ema_init 429450\<close>
+  \<open>ema_slow_init \<equiv> ema_init (429450)\<close> \<comment> \<open>2814749767\<close>
 
-text \<open>Small test below. It was useful once to detect an overflow that lead to very bad 
+text \<open>Small test below. It was useful once to detect an overflow that lead to very bad
   initialisation behaviour.\<close>
-value \<open>ema_get_value ( (((ema_update 12)^^ 1) (ema_init 128849010))) >> 32\<close>
 
+value \<open>let \<alpha> = shiftr 128849010 (EMA_FIXPOINT_SIZE - 32);
+        x =  (((ema_update 10)^^ 1) (7 * ema_bitshifting, \<alpha>, \<alpha>, 12, 12))
+  in (ema_extract_value x, ema_get_value x, x)\<close>
 
 end
