Weidenbach_Book/IsaSAT/IsaSAT_Options.thy
@@ -24,6 +24,8 @@ datatype opts =
   (opts_restart_coeff1: \<open>64 word\<close>)
   (opts_restart_coeff2: nat)
   (opts_target: \<open>opts_target\<close>)
+  (opts_fema: \<open>64 word\<close>)
+  (opts_sema: \<open>64 word\<close>)
 
 
 definition TARGET_NEVER :: \<open>opts_target\<close> where
@@ -39,12 +41,12 @@ definition TARGET_ALWAYS :: \<open>opts_target\<close> where
 subsection \<open>Refinement\<close>
 
 type_synonym opts_ref =
-  \<open>bool \<times> bool \<times> bool \<times> 64 word \<times> 64 word \<times> nat \<times> opts_target\<close>
+  \<open>bool \<times> bool \<times> bool \<times> 64 word \<times> 64 word \<times> nat \<times> opts_target \<times> 64 word \<times> 64 word\<close>
 
 definition opts_rel :: \<open>(opts_ref \<times> opts) set\<close> where
   \<open>opts_rel = {(S, T). S = (opts_restart T, opts_reduce T, opts_unbounded_mode T,
       opts_minimum_between_restart T, opts_restart_coeff1 T, opts_restart_coeff2 T,
-      opts_target T)}\<close>
+      opts_target T, opts_fema T, opts_sema T)}\<close>
 
 fun opts_rel_restart :: \<open>opts_ref \<Rightarrow> bool\<close> where
   \<open>opts_rel_restart (res, red, unbd, mini, res1, res2) = res\<close>
@@ -52,7 +54,6 @@ fun opts_rel_restart :: \<open>opts_ref \<Rightarrow> bool\<close> where
 lemma opts_rel_restart:
   \<open>(opts_rel_restart, opts_restart) \<in> opts_rel \<rightarrow> bool_rel\<close>
   by (auto simp: opts_rel_def intro!: frefI)
-
 
 fun opts_rel_reduce :: \<open>opts_ref \<Rightarrow> bool\<close> where
   \<open>opts_rel_reduce (res, red, unbd, mini, res1, res2) = red\<close>
@@ -90,10 +91,24 @@ lemma opts_rel_restart_coeff2:
   by (auto simp: opts_rel_def intro!: frefI)
 
 fun opts_rel_target :: \<open>opts_ref \<Rightarrow> 3 word\<close> where
-  \<open>opts_rel_target (res, red, unbd, mini, res1, res2, target) = target\<close>
+  \<open>opts_rel_target (res, red, unbd, mini, res1, res2, target, fema, sema) = target\<close>
 
 lemma opts_rel_target:
   \<open>(opts_rel_target, opts_target) \<in> opts_rel \<rightarrow> Id\<close>
+  by (auto simp: opts_rel_def intro!: frefI)
+
+fun opts_rel_fema :: \<open>opts_ref \<Rightarrow> 64 word\<close> where
+  \<open>opts_rel_fema (res, red, unbd, mini, res1, res2, target, fema, sema) = fema\<close>
+
+lemma opts_rel_fema:
+  \<open>(opts_rel_fema, opts_fema) \<in> opts_rel \<rightarrow> Id\<close>
+  by (auto simp: opts_rel_def intro!: frefI)
+
+fun opts_rel_sema :: \<open>opts_ref \<Rightarrow> 64 word\<close> where
+  \<open>opts_rel_sema (res, red, unbd, mini, res1, res2, target, fema, sema) = sema\<close>
+
+lemma opts_rel_sema:
+  \<open>(opts_rel_sema, opts_sema) \<in> opts_rel \<rightarrow> Id\<close>
   by (auto simp: opts_rel_def intro!: frefI)
 
 lemma opts_rel_alt_defs:
@@ -103,7 +118,9 @@ lemma opts_rel_alt_defs:
   \<open>RETURN o opts_rel_miminum_between_restart = (\<lambda>(res, red, unbd, mini, res1, res2). RETURN mini)\<close>
   \<open>RETURN o opts_rel_restart_coeff1 = (\<lambda>(res, red, unbd, mini, res1, res2). RETURN res1)\<close>
   \<open>RETURN o opts_rel_restart_coeff2 = (\<lambda>(res, red, unbd, mini, res1, res2, _). RETURN res2)\<close>
-  \<open>RETURN o opts_rel_target = (\<lambda>(res, red, unbd, mini, res1, res2, target). RETURN target)\<close>
+  \<open>RETURN o opts_rel_target = (\<lambda>(res, red, unbd, mini, res1, res2, target, fema, semax). RETURN target)\<close>
+  \<open>RETURN o opts_rel_fema = (\<lambda>(res, red, unbd, mini, res1, res2, target, fema, sema). RETURN fema)\<close>
+  \<open>RETURN o opts_rel_sema = (\<lambda>(res, red, unbd, mini, res1, res2, target, fema, sema). RETURN sema)\<close>
   by (auto intro!: ext)
 
 end
