Weidenbach_Book/IsaSAT/IsaSAT_Options_LLVM.thy
@@ -2,11 +2,12 @@ theory IsaSAT_Options_LLVM
   imports IsaSAT_Options IsaSAT_Literals_LLVM
 begin
 
-type_synonym opts_assn = \<open>1 word \<times> 1 word \<times> 1 word \<times> 64 word \<times> 64 word \<times> 64 word \<times> 3 word\<close>
+type_synonym opts_assn = \<open>1 word \<times> 1 word \<times> 1 word \<times> 64 word \<times> 64 word \<times> 64 word \<times> 3 word \<times> 64 word
+   \<times> 64 word\<close>
 
 definition opts_rel_assn :: \<open>opts_ref \<Rightarrow> _ \<Rightarrow> assn\<close> where
   \<open>opts_rel_assn = bool1_assn \<times>\<^sub>a bool1_assn \<times>\<^sub>a bool1_assn \<times>\<^sub>a word_assn \<times>\<^sub>a word_assn 
-   \<times>\<^sub>a snat_assn' TYPE(64) \<times>\<^sub>a word_assn' TYPE(3)\<close>
+   \<times>\<^sub>a snat_assn' TYPE(64) \<times>\<^sub>a word_assn' TYPE(3) \<times>\<^sub>a word64_assn \<times>\<^sub>a word64_assn\<close>
 
 sepref_def opts_rel_restart_code
   is \<open>RETURN o opts_rel_restart\<close>
@@ -51,6 +52,18 @@ sepref_def opts_rel_target_code
   unfolding opts_rel_alt_defs opts_rel_assn_def
   by sepref
 
+sepref_def opts_rel_fema_code
+  is \<open>RETURN o opts_rel_fema\<close>
+  :: \<open>opts_rel_assn\<^sup>k \<rightarrow>\<^sub>a word64_assn\<close>
+  unfolding opts_rel_alt_defs opts_rel_assn_def
+  by sepref
+
+sepref_def opts_rel_sema_code
+  is \<open>RETURN o opts_rel_sema\<close>
+  :: \<open>opts_rel_assn\<^sup>k \<rightarrow>\<^sub>a word64_assn\<close>
+  unfolding opts_rel_alt_defs opts_rel_assn_def
+  by sepref
+
 definition opts_assn :: \<open>opts \<Rightarrow> opts_assn \<Rightarrow> assn\<close> where
   \<open>opts_assn = hr_comp opts_rel_assn opts_rel\<close>
 
@@ -62,9 +75,11 @@ lemmas [sepref_fr_rules] =
   opts_rel_restart_coeff1_code.refine[FCOMP opts_rel_restart_coeff1, unfolded opts_assn_def[symmetric]]
   opts_rel_restart_coeff2_code.refine[FCOMP opts_rel_restart_coeff2, unfolded opts_assn_def[symmetric]]
   opts_rel_target_code.refine[FCOMP opts_rel_target, unfolded opts_assn_def[symmetric]]
+  opts_rel_fema_code.refine[FCOMP opts_rel_fema, unfolded opts_assn_def[symmetric]]
+  opts_rel_sema_code.refine[FCOMP opts_rel_sema, unfolded opts_assn_def[symmetric]]
 
 sepref_register opts_restart opts_reduce opts_minimum_between_restart opts_restart_coeff1
-  opts_restart_coeff2 opts_target
+  opts_restart_coeff2 opts_target opts_fema opts_sema
 
 lemma opts_assn_assn_pure[safe_constraint_rules]: \<open>CONSTRAINT is_pure opts_assn\<close>
   unfolding opts_assn_def opts_rel_assn_def
@@ -73,24 +88,24 @@ lemma opts_assn_assn_pure[safe_constraint_rules]: \<open>CONSTRAINT is_pure opts
 lemmas [sepref_frame_free_rules] = mk_free_is_pure[OF opts_assn_assn_pure[unfolded CONSTRAINT_def]]
 
 definition default_opts :: opts where
-  \<open>default_opts = IsaOptions True True True 50 11 4 1\<close>
+  \<open>default_opts = IsaOptions True True True 50 11 4 1 128849010 429450\<close>
 
 definition default_opts2 :: opts_ref where
-  \<open>default_opts2 = (True, True, True, 50, 11, 4, 2)\<close>
+  \<open>default_opts2 = (True, True, True, 50, 11, 4, 2, 128849010, 429450)\<close>
 
-definition IsaOptions_rel :: \<open>bool \<Rightarrow> bool \<Rightarrow> bool \<Rightarrow> 64 word \<Rightarrow> 64 word \<Rightarrow> nat \<Rightarrow> opts_target \<Rightarrow> opts_ref\<close> where
-  \<open>IsaOptions_rel a b c d e f g = (a, b, c, d, e, f, g)\<close>
+definition IsaOptions_rel :: \<open>bool \<Rightarrow> bool \<Rightarrow> bool \<Rightarrow> 64 word \<Rightarrow> 64 word \<Rightarrow> nat \<Rightarrow> opts_target \<Rightarrow> 64 word \<Rightarrow> 64 word \<Rightarrow> opts_ref\<close> where
+  \<open>IsaOptions_rel a b c d e f g h i = (a, b, c, d, e, f, g, h, i)\<close>
 
 lemma IsaOptions_rel:
-  \<open>(uncurry6 (RETURN ooooooo IsaOptions_rel), uncurry6 (RETURN ooooooo IsaOptions)) \<in>
-     bool_rel \<times>\<^sub>f bool_rel \<times>\<^sub>f  bool_rel \<times>\<^sub>f  word_rel \<times>\<^sub>f word_rel \<times>\<^sub>f nat_rel \<times>\<^sub>f word_rel \<rightarrow>
+  \<open>(uncurry8 (RETURN ooooooooo IsaOptions_rel), uncurry8 (RETURN ooooooooo IsaOptions)) \<in>
+     bool_rel \<times>\<^sub>f bool_rel \<times>\<^sub>f  bool_rel \<times>\<^sub>f  word_rel \<times>\<^sub>f word_rel \<times>\<^sub>f nat_rel \<times>\<^sub>f word_rel \<times>\<^sub>f word_rel \<times>\<^sub>f word_rel \<rightarrow>
      \<langle>opts_rel\<rangle>nres_rel\<close>
   by (auto intro!: frefI nres_relI simp: opts_rel_def IsaOptions_rel_def)
 
 sepref_def IsaOptions_rel_impl
-  is \<open>uncurry6 (RETURN ooooooo IsaOptions_rel)\<close>
+  is \<open>uncurry8 (RETURN ooooooooo IsaOptions_rel)\<close>
   :: \<open>bool1_assn\<^sup>k *\<^sub>a bool1_assn\<^sup>k *\<^sub>a bool1_assn\<^sup>k *\<^sub>a word_assn\<^sup>k *\<^sub>a word_assn\<^sup>k *\<^sub>a
-     (snat_assn' (TYPE(64)))\<^sup>k  *\<^sub>a (word_assn' (TYPE(3)))\<^sup>k \<rightarrow>\<^sub>a
+     (snat_assn' (TYPE(64)))\<^sup>k  *\<^sub>a (word_assn' (TYPE(3)))\<^sup>k  *\<^sub>a word_assn\<^sup>k  *\<^sub>a word_assn\<^sup>k \<rightarrow>\<^sub>a
         opts_rel_assn\<close>
   unfolding IsaOptions_rel_def opts_rel_assn_def
   by sepref
